backend/RTL.v
@@ -283,7 +283,7 @@ Inductive step: state -> trace -> state -> Prop :=
   | exec_function_internal:
       forall s f args m m' m'' stk sz,
       Mem.alloc m 0 f.(fn_stacksize) = (m', stk) ->
-      Mem.record_frame_vm m' (Mem.mk_frame sz) = Some m'' ->
+      Mem.record_frame m' (Mem.mk_frame sz) = Some m'' ->
       step (Callstate s (Internal f) args m sz)
         E0 (State s
                   f
