backend/RTLmachproof.v
@@ -44,7 +44,7 @@ Proof.
   unfold match_prog in TRANSL. unfold ge.
   unfold tge. congruence.
 Qed.
-
+(*
 Lemma stage_size_head_le_all : forall s : Mem.stage,
     Mem.size_of_head_frame s <= Mem.size_of_all_frames s.
 Proof.
@@ -61,7 +61,7 @@ Proof.
   - simpl. generalize (stage_size_head_le_all a).
     lia.
 Qed.
-
+*)
 Lemma find_function_translated:
   forall ros rs rs' f,
   find_function ge ros rs = Some f ->
@@ -92,61 +92,412 @@ Proof.
   - auto.
 Qed.
 
-Definition match_states (s1 s2:state) := s1 = s2.
-
-Lemma step_simulation:
-  forall S1 t S2, RTL.step fn_stack_requirements ge S1 t S2 ->
-  forall S1', match_states S1 S1' ->
-  exists S2', step fn_stack_requirements tge S1' t S2' /\ match_states S2 S2'.
+Lemma lessdef_list_refl : forall s,
+    Val.lessdef_list s s.
 Proof.
-  intros. inv H0. rewrite <- genv_eq. exists S2.
-  inv H; split.
-  constructor; auto. reflexivity.
-  econstructor; eauto. reflexivity.
-  eapply exec_Iload; eauto.  reflexivity.
-  eapply exec_Istore; eauto. reflexivity.
-  eapply exec_Icall; eauto. reflexivity.
-  econstructor; eauto. reflexivity.
-  econstructor; eauto. reflexivity.
-  eapply exec_Icond; eauto. reflexivity.
-  eapply exec_Ijumptable; eauto. reflexivity.
-  eapply exec_Ireturn; eauto. reflexivity.
-  econstructor. apply H0.
-  apply Mem.record_frame_vm_result in H1 as H2.
-  apply Mem.record_frame_vm_size in H1 as H3.
-  unfold Mem.record_frame_mach. rewrite H2.
-  generalize (stack_size_mach_le_vm (Mem.stack (Mem.support m''))).
-  intro.
-  assert (Mem.stack_size_mach (Mem.stack (Mem.support m'')) <= Mem.max_stacksize) by lia.
-  apply zle_true. auto. reflexivity.
-  econstructor; eauto. reflexivity.
-  econstructor; eauto. reflexivity.
+  induction s; eauto.
+Qed.
+Inductive match_stackadt : Mem.stackadt -> Mem.stackadt -> Prop :=
+  |match_stackadt_nil : match_stackadt nil nil
+  |match_stackadt_cons : forall s1 s2 (t1:Mem.stage) (t1':Mem.stage) (frame:Mem.frame),
+     match_stackadt s1 s2 ->
+     t1 = frame::t1' ->
+     match_stackadt (t1::s1) ((frame::nil)::s2).
+
+Lemma match_stackadt_size : forall s1 s2,
+    match_stackadt s1 s2 ->
+    Mem.stack_size s2 <= Mem.stack_size s1.
+Proof.
+  intros. induction H.
+  - lia.
+  - simpl. rewrite H0. simpl in *.
+    generalize (Mem.size_of_all_frames_pos t1').
+    lia.
 Qed.
 
-Lemma transl_initial_states:
-  forall S, RTL.initial_state fn_stack_requirements prog S ->
-  exists R, initial_state fn_stack_requirements tprog R /\ match_states S R.
-Proof.
-  intros. exists S. split. inv TRANSL.
-  inv H. econstructor; eauto. reflexivity.
+
+
+(*
+Lemma valid_pointer_memiff : forall m1 m2 b ofs,
+    mem_iff m1 m2 -> Mem.valid_pointer m1 b ofs = true <-> Mem.valid_pointer m2 b ofs = true.
+Proof. intros. inv H.
+       transitivity (Mem.perm m1 b ofs Cur Nonempty).
+       apply Mem.valid_pointer_nonempty_perm.
+       transitivity (Mem.perm m2 b ofs Cur Nonempty).
+       unfold Mem.perm. rewrite perm_iff0. reflexivity.
+       symmetry.        apply Mem.valid_pointer_nonempty_perm.
 Qed.
 
-Lemma transl_final_states:
-  forall S R r,
-  match_states S R -> RTL.final_state S r -> final_state R r.
-Proof.
-  intros. inv H0. inv H. constructor.
+Lemma valid_pointer_memiff1 : forall m1 m2 b ofs,
+    mem_iff m1 m2 -> Mem.valid_pointer m1 b ofs = Mem.valid_pointer m2 b ofs.
+Proof. intros.
+       destruct (Mem.valid_pointer m1 b ofs) eqn:vp1.
+       generalize (valid_pointer_memiff _ _ b ofs H). intros.
+       apply H0 in vp1. rewrite vp1. auto.
+       destruct (Mem.valid_pointer m2 b ofs) eqn:vp2.
+       eapply valid_pointer_memiff in vp2; eauto. auto.
 Qed.
 
-Theorem transf_program_correct:
-  forward_simulation (RTL.semantics fn_stack_requirements prog)
-                     (semantics fn_stack_requirements tprog).
+Lemma eval_cond_memiff:
+    forall  (m m0 : mem) (cond : condition) (vl : list val),
+      mem_iff m m0 ->
+      eval_condition cond vl m0 =
+      eval_condition cond vl m.
 Proof.
-  eapply forward_simulation_step.
-  inv TRANSL. auto.
-  eexact transl_initial_states.
-  eexact transl_final_states.
-  exact step_simulation.
+    intros m m0 cond vl H6.
+    unfold eval_condition. destruct cond; auto.
+    unfold Val.cmplu_bool. repeat destr.
+    repeat (erewrite (valid_pointer_memiff1 m m0 _ _) in Heqb2; eauto). congruence.
+    repeat (erewrite (valid_pointer_memiff1 m m0 _ _) in Heqb2; eauto). congruence.
+    repeat (erewrite (valid_pointer_memiff1 m m0 _ _) in Heqb2; eauto). congruence.
+    repeat (erewrite (valid_pointer_memiff1 m m0 _ _) in Heqb2; eauto). congruence.
+    repeat (erewrite (valid_pointer_memiff1 m m0 _ _) in Heqb2; eauto). congruence.
+    repeat (erewrite (valid_pointer_memiff1 m m0 _ _) in Heqb2; eauto). congruence.
+    repeat (erewrite (valid_pointer_memiff1 m m0 _ _) in Heqb2; eauto). congruence.
+    repeat (erewrite (valid_pointer_memiff1 m m0 _ _) in Heqb2; eauto). congruence.
+    unfold Val.cmplu_bool. repeat destr.
+    repeat (erewrite (valid_pointer_memiff1 m m0 _ _) in Heqb2; eauto). congruence.
+    repeat (erewrite (valid_pointer_memiff1 m m0 _ _) in Heqb2; eauto). congruence.
 Qed.
+Lemma eval_op_memiff:
+  forall (sp : val) (m m0 : mem) (op : operation)
+    (vl :list val) (v : val) (H3 : eval_operation ge sp op vl m = Some v)
+    (H6 : mem_iff m m0), eval_operation ge sp op vl m0 = Some v.
+Proof.
+  intros sp m m0 op vl v H3 H6.
+  unfold eval_operation in *. destruct op; auto.
+  erewrite eval_cond_memiff; eauto.
+  repeat destr.
+  erewrite eval_cond_memiff; eauto.
+Qed.
+
+Lemma eval_builtin_args_memiff:
+  forall (sp : val) (rs : Regmap.t val) (m m0 : mem) (args : list (builtin_arg reg))
+    (vargs : list val) (H3 : eval_builtin_args ge (fun r : positive => rs # r) sp m args vargs)
+    (H7 : mem_iff m m0),
+    eval_builtin_args ge (fun r : positive => rs # r) sp m0 args vargs.
+Proof.
+  intros sp rs m m0 args vargs H3 H7. Admitted. (*loadv_memiff needed*)
+
+Inductive match_states: RTL.state -> RTL.state -> Prop :=
+  | match_regular_states: forall stk f sp pc rs m m',
+        mem_iff m' m ->
+        match_stackadt (Mem.stack(Mem.support m)) (Mem.stack(Mem.support m'))->
+      match_states (State stk f sp pc rs m)
+                   (State stk f sp pc rs m')
+  | match_callstates: forall stk f args m sz m' hd tl,
+        mem_iff m' m ->
+        Mem.stack(Mem.support m) = hd :: tl ->
+        match_stackadt tl (Mem.stack(Mem.support m')) ->
+      match_states (Callstate stk f args m sz)
+                   (Callstate stk f args m' sz)
+  | match_returnstates: forall stk v  m m' hd tl,
+        mem_iff m' m ->
+        Mem.stack(Mem.support m) = hd :: tl ->
+        match_stackadt tl (Mem.stack(Mem.support m')) ->
+      match_states (Returnstate stk v m)
+                   (Returnstate stk v m').
+
+Lemma storev_memiff:
+  forall (rs : Regmap.t val) (m m0 : mem) (chunk : memory_chunk) (src : reg)
+    (a : val) (m' : mem) (H4 : Mem.storev chunk m a rs # src = Some m')
+    (H7 : mem_iff m m0),
+    exists m'0,
+    Mem.storev chunk m0 a rs # src = Some m'0/\mem_iff m' m'0.
+Proof.
+  intros rs m m0 chunk src a m' H4 H7. Admitted.
+
+Lemma backward_simulation_step:
+  forall S1' t S2', step fn_stack_requirements ge S1' t S2' ->
+  forall S1, match_states S1 S1' -> safe (RTL.semantics fn_stack_requirements prog) S1 ->
+  exists S2, plus (RTL.step fn_stack_requirements) ge S1 t S2 /\ match_states S2 S2'.
+Proof.
+  intros. inv H; inv H0.
+  - econstructor; eauto. split.
+    apply plus_one. econstructor; eauto.
+    econstructor; eauto.
+  - econstructor; eauto. split.
+    apply plus_one. eapply RTL.exec_Iop; eauto.
+    eapply eval_op_memiff; eauto.
+    econstructor; eauto.
+  - econstructor; eauto. split. apply plus_one.
+    eapply RTL.exec_Iload; eauto.
+    eapply loadv_memiff; eauto.
+    econstructor; eauto.
+  - exploit storev_memiff; eauto. intros [m0' [STOREV IFF]].
+    econstructor; eauto. split. apply plus_one.
+    eapply RTL.exec_Istore; eauto.
+    econstructor; eauto.
+    rewrite <- (Mem.support_storev _ _ _ _ _ H4).
+    rewrite <- (Mem.support_storev _ _ _ _ _ STOREV).
+    auto.
+  - econstructor; eauto. split. apply plus_one.
+    eapply RTL.exec_Icall; eauto.
+    econstructor; eauto. (*push_left*)
+    admit. reflexivity.
+  - econstructor; eauto. split. apply plus_one.
+    eapply RTL.exec_Itailcall; eauto.
+    admit. (*free parallel pop_left*)
+    econstructor; eauto. admit. admit. admit.
+(*
+    destruct H7 as [hd H7].
+    rewrite <- (Mem.support_free _ _ _ _ _ FREE) in H16.
+    rewrite <- (Mem.support_free _ _ _ _ _ H6) in H16.
+    rewrite S2 in H16. rewrite H7 in H16. inv H16.
+    auto. *)
+  - (*push right*)
+     econstructor; eauto. split. apply plus_one.
+     econstructor; eauto.
+*)     
+  
+
+Inductive match_stackframes: list stackframe -> list stackframe -> Prop :=
+  | match_stackframes_nil:
+      match_stackframes nil nil
+  | match_stackframes_normal: forall stk stk' res sp pc rs rs' f,
+      match_stackframes stk stk' ->
+      regs_lessdef rs rs' ->
+      match_stackframes
+        (Stackframe res f sp pc rs :: stk)
+        (Stackframe res f sp pc rs' :: stk').
+
+Inductive match_states: RTL.state -> RTL.state -> Prop :=
+  | match_regular_states: forall stk stk' f sp pc rs rs' m m',
+        regs_lessdef rs' rs ->
+        Mem.extends' m' m ->
+        match_stackframes stk' stk ->
+        match_stackadt (Mem.stack(Mem.support m)) (Mem.stack(Mem.support m'))->
+      match_states (State stk f sp pc rs m)
+                   (State stk' f sp pc rs' m')
+  | match_callstates: forall stk stk' f args args' m sz m' hd tl,
+        Val.lessdef_list args' args->
+        Mem.extends' m' m ->
+        match_stackframes stk' stk ->
+        Mem.stack(Mem.support m) = hd :: tl ->
+        match_stackadt tl (Mem.stack(Mem.support m')) ->
+      match_states (Callstate stk f args m sz)
+                   (Callstate stk' f args' m' sz)
+  | match_returnstates: forall stk stk' v v' m m' hd tl,
+        Val.lessdef v' v ->
+        Mem.extends' m' m ->
+        match_stackframes stk' stk ->
+        Mem.stack(Mem.support m) = hd :: tl ->
+        match_stackadt tl (Mem.stack(Mem.support m')) ->
+      match_states (Returnstate stk v m)
+                   (Returnstate stk' v' m').
+
+
+Lemma regs_lessdef_init_regs:
+  forall params vl vl',
+  Val.lessdef_list vl vl' ->
+  regs_lessdef (init_regs vl params) (init_regs vl' params).
+Proof.
+  induction params; intros.
+  simpl. red; intros. rewrite Regmap.gi. constructor.
+  simpl. inv H.   red; intros. rewrite Regmap.gi. constructor.
+  apply set_reg_lessdef. auto. auto.
+Qed.
+
+Lemma backward_simulation_step:
+  forall S1' t S2', step fn_stack_requirements ge S1' t S2' ->
+  forall S1, match_states S1 S1' -> safe (RTL.semantics fn_stack_requirements prog) S1 ->
+  exists S2, plus (RTL.step fn_stack_requirements) ge S1 t S2 /\ match_states S2 S2'.
+Proof.
+  intros. inv H; inv H0.
+  - econstructor; eauto. split.
+    apply plus_one. econstructor; eauto.
+    econstructor; eauto.
+  - assert (Val.lessdef_list (rs##args) (rs0##args)). apply regs_lessdef_regs; auto.
+    exploit eval_operation_lessdef; eauto.
+    intros [v' [EVAL' VLD]].
+    econstructor; eauto. split.
+    apply plus_one. eapply RTL.exec_Iop; eauto.
+    econstructor; eauto. apply set_reg_lessdef; eauto.
+  - assert (Val.lessdef_list (rs##args) (rs0##args)). apply regs_lessdef_regs; auto.
+    exploit eval_addressing_lessdef; eauto.
+    intros [v' [EVAL' VLD]].
+    exploit Mem.loadv_extends'; eauto.
+    intros [v'' [LOAD VLD']].
+    econstructor; eauto. split. apply plus_one.
+    eapply RTL.exec_Iload; eauto.
+    econstructor; eauto. intro.
+    apply set_reg_lessdef; eauto.
+  - assert (Val.lessdef_list (rs##args) (rs0##args)). apply regs_lessdef_regs; auto.
+    exploit eval_addressing_lessdef; eauto.
+    intros [v' [EVAL' VLD]].
+    exploit Mem.storev_extends'; eauto.
+    intros [m2' [STORE VLD']].
+    econstructor; eauto. split. apply plus_one.
+    eapply RTL.exec_Istore; eauto.
+    econstructor; eauto.
+    rewrite <- (Mem.support_storev _ _ _ _ _ H4).
+    rewrite <- (Mem.support_storev _ _ _ _ _ STORE).
+    auto.
+  - econstructor; eauto. split. apply plus_one.
+    eapply RTL.exec_Icall; eauto.
+    eapply find_function_id_preserved; eauto.
+    eapply find_function_translated; eauto.
+    eapply match_callstates; eauto. apply regs_lessdef_regs. auto.
+    2: constructor; auto.
+    2: constructor; auto.
+    {
+      inv H12. constructor; simpl; eauto. inv mext_inj.
+      constructor; eauto.
+    }
+  - exploit Mem.free_parallel_extends'; eauto.
+    intros [m2' [FREE EXT]].
+      destruct (Mem.stack(Mem.support m2')) eqn : S2.
+        apply Mem.support_free in FREE. rewrite <- FREE in H16.
+        rewrite S2 in H16. inv H16.
+        apply Mem.pop_stage_nonempty in H7.
+        erewrite Mem.support_free in H7; eauto. congruence.
+    econstructor; eauto. split. apply plus_one.
+    eapply RTL.exec_Itailcall; eauto.
+    eapply find_function_id_preserved; eauto.
+    eapply find_function_translated; eauto.
+    eapply match_callstates; eauto. apply regs_lessdef_regs. auto.
+    eapply Mem.pop_stage_left_extends'; eauto.
+    eapply Mem.stack_pop_stage in H7.
+    destruct H7 as [hd H7].
+    rewrite <- (Mem.support_free _ _ _ _ _ FREE) in H16.
+    rewrite <- (Mem.support_free _ _ _ _ _ H6) in H16.
+    rewrite S2 in H16. rewrite H7 in H16. inv H16.
+    auto.
+  - exploit (@eval_builtin_args_lessdef _ ge (fun r => rs#r) (fun r => rs0#r)); eauto.
+    intros (vargs' & P & Q).
+    assert (Mem.extends' m (Mem.push_stage m0)).
+    {
+      inv H12. constructor; simpl; eauto. inv mext_inj.
+      constructor; eauto.
+    }
+    exploit external_call_mem_extends'. 2: apply H. all:eauto.
+    intros [v' [m'1 [A [B [C D]]]]].
+    apply external_call_mem_stackeq in A as A'.
+    assert ({m'2:mem|Mem.pop_stage m'1 = Some m'2}).
+      apply Mem.nonempty_pop_stage.
+      rewrite <- A'. simpl. congruence.
+    destruct X as [m'2 POP].
+    econstructor; eauto. split. apply plus_one.
+    eapply RTL.exec_Ibuiltin; eauto.
+    econstructor; eauto. apply set_res_lessdef; auto.
+    eapply Mem.pop_stage_right_extends'; eauto.
+    erewrite <- (external_call_mem_stackeq _ _ _ _ _ _ _ H4).
+    apply Mem.stack_pop_stage in POP. destruct POP as [hd POP].
+    rewrite <- A' in POP. simpl in POP. inv POP.
+    auto.
+  - exists (State stk f sp (if b then ifso else ifnot) rs0 m0); split.
+    apply plus_one. eapply RTL.exec_Icond; eauto.
+    apply eval_condition_lessdef with (rs##args) m; auto. apply regs_lessdef_regs; auto.
+    econstructor; eauto.
+  - exists (State stk f sp pc' rs0 m0); split.
+    apply plus_one. eapply RTL.exec_Ijumptable; eauto.
+    generalize (H9 arg). rewrite H3. intro. inv H. auto.
+    econstructor; eauto.
+  - exploit Mem.free_parallel_extends'; eauto.
+    intros [m2' [FREE EXT]].
+    apply Mem.stack_pop_stage in H4 as H4'.
+    destruct H4' as [hd H4'].
+    rewrite <- (Mem.support_free _ _ _ _ _ H3) in H14.
+    rewrite H4' in H14.
+    inv H14.
+    exists (Returnstate stk0 (regmap_optget or Vundef rs0) m2'); split.
+    apply plus_one. eapply RTL.exec_Ireturn; eauto.
+    econstructor; eauto.
+    destruct or; simpl. apply H9. constructor.
+    eapply Mem.pop_stage_left_extends'; eauto.
+    rewrite (Mem.support_free _ _ _ _ _ FREE). inv H. reflexivity.
+  - red in H1. generalize (H1 (Callstate stk0 (Internal f )args0 m0 sz)). intros.
+    exploit H. apply star_refl. intros [Sf|Sf].
+    + destruct Sf as [r Sf]. inv Sf.
+    + destruct Sf as (E & s'' & STEP).
+      exists s''. split. apply plus_one. simpl in STEP. unfold ge.
+      inv STEP. econstructor. eauto. eauto.
+      inv STEP.
+      exploit Mem.alloc_extends'; eauto.
+      instantiate (1 := 0). lia.
+      instantiate (1 := fn_stacksize f). lia.
+      intros (m'1 & ALLOC & EXT).
+      rewrite H15 in ALLOC. inv ALLOC.
+      eapply match_regular_states.
+      apply regs_lessdef_init_regs. auto.
+      eapply Mem.push_stage_left_extends' in EXT; eauto.
+    exploit Mem.record_frame_safe_extends'; eauto. auto.
+    apply Mem.stack_record_frame in H3 as STK1.
+    apply Mem.stack_record_frame in H16 as STK2.
+    destruct STK2 as (hd2 & tl2 & STKm'1 & STKm''0).
+    rewrite (Mem.support_alloc _ _ _ _ _ H15) in STKm'1.
+    simpl in STKm'1. rewrite H12 in STKm'1. inv STKm'1.
+    rewrite STKm''0.
+    destruct STK1 as (hd1 & tl1 & STKpm' & STKm'').
+    simpl in STKpm'. inv STKpm'. rewrite  STKm''.
+    apply Mem.support_alloc in H2. simpl in H2.
+    rewrite H2. simpl.
+    inv H13.
+    * econstructor. constructor. eauto.
+    * econstructor. econstructor. eauto. eauto. eauto.
+  -  exploit external_call_mem_extends'; eauto.
+    intros [v' [m1 [A [B [C D]]]]].
+    econstructor. split.
+    apply plus_one. econstructor. eauto.
+    econstructor; eauto.
+    erewrite <- external_call_mem_stackeq; eauto.
+    erewrite <- external_call_mem_stackeq; eauto.
+  - assert ({m1:mem|Mem.pop_stage m0 = Some m1}).
+      apply Mem.nonempty_pop_stage. congruence.
+      destruct X as [m1 POP].
+    inv H7.
+    econstructor. split. apply plus_one.
+    eapply RTL.exec_return; eauto.
+    econstructor; eauto. apply set_reg_lessdef; auto.
+    eapply Mem.pop_stage_right_extends'; eauto.
+    destruct (Mem.stack_pop_stage   _ _ POP).
+    rewrite H in H8. inv H8. auto.
+Qed.
+
+Definition initial_states_exist:
+  forall s1, RTL.initial_state fn_stack_requirements prog s1 ->
+             exists s2, initial_state fn_stack_requirements prog s2.
+Proof.
+  intros. inv TRANSL. inv H.
+  exists (Callstate nil f nil m0 (fn_stack_requirements (prog_main tprog))).
+  econstructor; eauto.
+Qed.
+
+Definition match_initial_states:
+  forall s1 s2, RTL.initial_state fn_stack_requirements prog s1 ->
+                initial_state fn_stack_requirements tprog s2 ->
+  exists s1', RTL.initial_state fn_stack_requirements prog s1' /\ match_states s1' s2.
+Proof.
+  intros. exists s1. split. auto.
+  inv H. inv H0.
+  rewrite prog_eq in *.    subst ge0. subst ge1.
+  rewrite prog_eq in *.
+  rewrite H2 in H5. inv H5.
+  rewrite H3 in H6. inv H6.
+  rewrite H1 in H. inv H.
+  eapply match_callstates; eauto.
+  eapply Mem.push_stage_right_extends'; eauto. apply Mem.extends'_refl.
+  constructor. simpl. reflexivity.
+  apply Genv.init_mem_stack in H1. rewrite H1.
+  constructor.
+Qed.
+
+Definition match_final_states:
+  forall s1 s2 r,
+  match_states s1 s2 -> final_state s2 r -> RTL.final_state s1 r.
+Proof.
+  intros. inv H0. inv H. inv H6. inv H3. inv H7.
+  constructor.
+Qed.
+Definition progress:
+  forall s1 s2,
+  match_states s1 s2 -> safe (RTL.semantics fn_stack_requirements prog) s1 ->
+  (exists r, RTL.final_state s2 r) \/
+  (exists t, exists s2', (step fn_stack_requirements) tge s2 t s2').
+Proof.
+  Admitted.
 
 End PRESERVATION.
+
+
+
