backend/RTLgenproof.v
@@ -1578,7 +1578,7 @@ Proof.
     exploit (add_vars_valid (CminorSel.fn_params f)); eauto. intros [A B].
     eapply add_vars_wf; eauto. eapply add_vars_wf; eauto. apply init_mapping_wf.
   edestruct Mem.alloc_extends as [tm' []]; eauto; try apply Z.le_refl.
-  edestruct Mem.record_frame_vm_extends as [tm'' []]; eauto.
+  edestruct Mem.record_frame_extends as [tm'' []]; eauto.
   econstructor; split.
   left; apply plus_one. eapply exec_function_internal; simpl; eauto.
   simpl. econstructor; eauto.
